updates

src/EvalExecs/Constructor.v
@@ -2,56 +2,18 @@ Require Import UrsusEnvironment.Solidity.current.Environment.
 Require Import UrsusEnvironment.Solidity.current.LocalGenerator.
 
 Require Import UMLang.ExecGenerator.
+Require Import Common.
 
 Require Import EIP20.
 Import EIP20.
 
-#[global, program]
-Instance listInfinite : listInfiniteFunRec_gen XList.
-Next Obligation.
-(* TODO: we need to analyze all while/for cycles
-   and find upper bound for number of iterations *)
-exact (repeat PhantomPoint 0).
-Defined.
-
-Notation rec := LocalStateLRecord.
-
-Definition computed : LocalStateLRecord := Eval vm_compute in default. 
-#[global]
-Instance def : XDefault LocalStateLRecord := {
-  default := computed 
-} . 
-
-Definition VMStateDefault : VMStateLRecord  := Eval vm_compute in default.
-Definition LedgerDefault : LedgerLRecord LocalStateLRecord  := Eval vm_compute in default. 
-
-Elpi Accumulate rec_def lp:{{
-  get_rec {{ rec }}.
-  get_def {{ def }}.
-}}.
-
-(* Definition msg_pubkey_right (rec: Type) (def: XDefault rec) := msg_pubkey.
-
-Check  msg_sender.
-
-Definition msg_sender_right (rec: Type) (def: XDefault rec) := msg_sender.
-Check  msg_sender_right.
-
-
-Definition msg_value_right (rec: Type) (def: XDefault rec) := msg_value.
-Definition tvm_pubkey_right (rec: Type) (def: XDefault rec) := tvm_pubkey.
-Definition _now_right (rec: Type) (def: XDefault rec) := \\ now \\.
- *)
-
-Check constructor.
 
 Definition constructor_exec_sig (_initialAmount :  uint256) 
                                 (_tokenName :  string) 
                                 (_decimalUnits :  uint8) 
                                 (_tokenSymbol :  string) (l : LedgerLRecord rec) :
                                 {t | t = exec_state (Uinterpreter (@constructor rec def _ _ _ _initialAmount _tokenName _decimalUnits _tokenSymbol)) l}.
-  unfold constructor. unfold dynamicAssignL.
-  (* unfold totalSupply_left, balances_left, name_left, symbol_left, decimals_left. *)
+  unfold constructor. unfold dynamicAssignL.  
   repeat auto_build_P listInfinite.
 Defined.
 
@@ -61,8 +23,6 @@ Definition constructor_exec_let (_initialAmount :  uint256)
                                 (_tokenSymbol :  string) (l : LedgerLRecord rec) : LedgerLRecord rec.
   let_term_of_2 @constructor_exec_sig (constructor_exec_sig _initialAmount _tokenName _decimalUnits _tokenSymbol l).
 Defined.
-
-(* Print constructor_exec_let. *)
 
 Definition constructor_exec (_initialAmount :  uint256) 
                             (_tokenName :  string) 
