src/EvalExecs/Transfer.v
@@ -2,33 +2,12 @@ Require Import UrsusEnvironment.Solidity.current.Environment.
 Require Import UrsusEnvironment.Solidity.current.LocalGenerator.
 
 Require Import UMLang.ExecGenerator.
+Require Import Common.
 
 Require Import EIP20.
 Import EIP20.
 
-#[global, program]
-Instance listInfinite : listInfiniteFunRec_gen XList.
-Next Obligation.
-(* TODO: we need to analyze all while/for cycles
-   and find upper bound for number of iterations *)
-exact (repeat PhantomPoint 0).
-Defined.
-
-Notation rec := LocalStateLRecord.
-
-Definition computed : LocalStateLRecord := Eval vm_compute in default. 
-#[global]
-Instance def : XDefault LocalStateLRecord := {
-  default := computed 
-} . 
-
-Definition VMStateDefault : VMStateLRecord  := Eval vm_compute in default.
-Definition LedgerDefault : LedgerLRecord LocalStateLRecord  := Eval vm_compute in default. 
-
-Elpi Accumulate rec_def lp:{{
-  get_rec {{ rec }}.
-  get_def {{ def }}.
-}}.
+(* exec *)
 
 Definition transfer_exec_sig (_to :  address) 
                              (_value :  uint256) (l : LedgerLRecord rec) :
@@ -42,8 +21,6 @@ Definition transfer_exec_let (_to :  address)
   let_term_of_2 @transfer_exec_sig (transfer_exec_sig _to _value l).
 Defined.
 
-(* Print constructor_exec_let. *)
-
 Definition transfer_exec (_to :  address) 
                          (_value :  uint256)  (l : LedgerLRecord rec) : LedgerLRecord rec.
   flat_term_of_2 @transfer_exec_let (transfer_exec_let _to _value l).
@@ -56,7 +33,7 @@ Definition transfer_exec_prf (_to :  address)
   proof_of_2 transfer_exec transfer_exec_sig (transfer_exec_sig _to _value l).
 Defined.
 
-
+(* eval *)
 
 Definition transfer_eval_sig (_to :  address) 
                              (_value :  uint256) (l : LedgerLRecord rec) :
@@ -71,14 +48,10 @@ Definition transfer_eval_let (_to :  address)
   let_term_of_2 @transfer_eval_sig (transfer_eval_sig _to _value l).
 Defined.
 
-(* Print constructor_exec_let. *)
-
 Definition transfer_eval (_to :  address) 
                          (_value :  uint256)  (l : LedgerLRecord rec) : ControlResult bool true.
   flat_term_of_2 @transfer_eval_let (transfer_eval_let _to _value l).
 Defined.
-
-Print transfer_eval.
 
 Definition transfer_eval_prf (_to :  address) 
                          (_value :  uint256) (l : LedgerLRecord rec) :
