src/EvalExecs/TransferFrom.v
@@ -2,46 +2,12 @@ Require Import UrsusEnvironment.Solidity.current.Environment.
 Require Import UrsusEnvironment.Solidity.current.LocalGenerator.
 
 Require Import UMLang.ExecGenerator.
+Require Import Common.
 
 Require Import EIP20.
 Import EIP20.
 
-#[global, program]
-Instance listInfinite : listInfiniteFunRec_gen XList.
-Next Obligation.
-(* TODO: we need to analyze all while/for cycles
-   and find upper bound for number of iterations *)
-exact (repeat PhantomPoint 0).
-Defined.
-
-Notation rec := LocalStateLRecord.
-
-Definition computed : LocalStateLRecord := Eval vm_compute in default. 
-#[global]
-Instance def : XDefault LocalStateLRecord := {
-  default := computed 
-} . 
-
-Definition VMStateDefault : VMStateLRecord  := Eval vm_compute in default.
-Definition LedgerDefault : LedgerLRecord LocalStateLRecord  := Eval vm_compute in default. 
-
-Elpi Accumulate rec_def lp:{{
-  get_rec {{ rec }}.
-  get_def {{ def }}.
-}}.
-
-(* Definition msg_pubkey_right (rec: Type) (def: XDefault rec) := msg_pubkey.
-
-Check  msg_sender.
-
-Definition msg_sender_right (rec: Type) (def: XDefault rec) := msg_sender.
-Check  msg_sender_right.
-
-
-Definition msg_value_right (rec: Type) (def: XDefault rec) := msg_value.
-Definition tvm_pubkey_right (rec: Type) (def: XDefault rec) := tvm_pubkey.
-Definition _now_right (rec: Type) (def: XDefault rec) := \\ now \\.
- *)
+(* exec *)
 
 Definition transferFrom_exec_sig (_from :  address)
                              (_to :  address) 
@@ -57,60 +23,11 @@ Definition transferFrom_exec_let (_from :  address)
   let_term_of_2 @transferFrom_exec_sig (transferFrom_exec_sig _from _to _value l).
 Defined.
 
-(* Print constructor_exec_let. *)
-
-Lemma exec_if_transit: forall X (b: bool) (f: LedgerT X) (x y: LedgerLRecord rec), 
-  exec_state f (if b then x else y) = if b then exec_state f x else exec_state f y.
-Proof.
-  intros.
-  destruct b; auto.
-Qed.
-
-Lemma exec_if_transit2: forall X (b: bool) (f: LedgerT X) (x y: LedgerLRecord rec), 
-  exec_state f (xBoolIfElse b x y) = if b then exec_state f x else exec_state f y.
-Proof.
-  intros.
-  destruct b; auto.
-Qed.
-
-Lemma eval_if_transit: forall X (b: bool) (f: LedgerT X) (x y: LedgerLRecord rec), 
-  eval_state f (if b then x else y) = if b then eval_state f x else eval_state f y.
-Proof.
-  intros.
-  destruct b; auto.
-Qed.
-
-Lemma eval_if_transit2: forall X (b: bool) (f: LedgerT X) (x y: LedgerLRecord rec), 
-  eval_state f (xBoolIfElse b x y) = if b then eval_state f x else eval_state f y.
-Proof.
-  intros.
-  destruct b; auto.
-Qed.
-
 Definition transferFrom_exec (_from :  address)
                          (_to :  address) 
                          (_value :  uint256)  (l : LedgerLRecord rec) : LedgerLRecord rec.
   flat_term_of_2 @transferFrom_exec_let (transferFrom_exec_let _from _to _value l).
 Defined.
-
-(* Print transferFrom_exec. *)
-
-(* Definition transferFrom_exec2 (_from :  address)
-                         (_to :  address) 
-                         (_value :  uint256)  (l : LedgerLRecord rec) : LedgerLRecord rec.
-remember (transferFrom_exec _from _to _value l).
-unfold transferFrom_exec in Heql0.
-(* symmetry in Heql0. *)
-repeat rewrite exec_if_transit, exec_if_transit2 in Heql0.
-match goal with 
-| Heql0: l0 = ?l |- _ => exact l
-end.
-Defined. *)
-
-
-(* Print transferFrom_exec2. *)
-
-
 
 Definition transferFrom_prf (_from :  address)
                          (_to :  address) 
@@ -120,5 +37,35 @@ Definition transferFrom_prf (_from :  address)
   proof_of_2 transferFrom_exec transferFrom_exec_sig (transferFrom_exec_sig _from _to _value l).
 Defined.
 
+(* Definition transferFrom_let_prf (_from :  address)
+                         (_to :  address) 
+                         (_value :  uint256) (l : LedgerLRecord rec) :
+  transferFrom_exec_let _from _to _value l = 
+  exec_state (Uinterpreter (@transferFrom rec def _ _ _ _ _from _to _value)) l.
+  proof_of_2 transferFrom_exec_let transferFrom_exec_sig (transferFrom_exec_sig _from _to _value l).
+Defined. *)
 
-(* Print transferFrom_exec. *)
+Definition transferFrom_eval_sig (_from :  address) (_to :  address) 
+                             (_value :  uint256) (l : LedgerLRecord rec) :
+                             {t | t = eval_state (Uinterpreter (@transferFrom rec def _ _ _ _  _from _to _value)) l}.
+  unfold transferFrom. unfold dynamicAssignL.
+  unfold fromUReturnExpression.  
+  repeat auto_build_P listInfinite.
+Defined.
+
+Definition transferFrom_eval_let (_from :  address) (_to :  address) 
+                             (_value :  uint256) (l : LedgerLRecord rec) : ControlResult bool true.
+  let_term_of_2 @transferFrom_eval_sig (transferFrom_eval_sig _from _to _value l).
+Defined.
+
+Definition transferFrom_eval (_from :  address) (_to :  address) 
+                         (_value :  uint256)  (l : LedgerLRecord rec) : ControlResult bool true.
+  flat_term_of_2 @transferFrom_eval_let (transferFrom_eval_let _from _to _value l).
+Defined.
+
+Definition transferFrom_eval_prf (_from :  address) (_to :  address) 
+                         (_value :  uint256) (l : LedgerLRecord rec) :
+  transferFrom_eval _to _value l = 
+  eval_state (Uinterpreter (@transferFrom rec def _ _ _ _ _from _to _value)) l.
+  proof_of_2 transferFrom_eval transferFrom_eval_sig (transferFrom_eval_sig _from _to _value l).
+Defined.
