src/Proofs/Constructor.v
@@ -3,67 +3,83 @@ Require Import UrsusEnvironment.Solidity.current.LocalGenerator.
 Require Import FinProof.Lib.HMapList.
 
 Require Import UMLang.ExecGenerator.
+Require Import Common.
 
 Require Import EIP20.
 Import EIP20.
 
 Require Import EvalExecs.Constructor.
 
-#[local]
-Existing Instance BoolEq.pair_eqb_spec.
-
-
-#[global, program]
-Instance listInfinite : listInfiniteFunRec_gen XList.
-Next Obligation.
-(* TODO: we need to analyze all while/for cycles
-   and find upper bound for number of iterations *)
-exact (repeat PhantomPoint 0).
-Defined.
-
-Notation rec := LocalStateLRecord.
-
-Definition computed : LocalStateLRecord := Eval vm_compute in default. 
-#[global]
-Instance def : XDefault LocalStateLRecord := {
-  default := computed 
-} . 
-
-Definition VMStateDefault : VMStateLRecord  := Eval vm_compute in default.
-Definition LedgerDefault : LedgerLRecord LocalStateLRecord  := Eval vm_compute in default. 
-
-Elpi Accumulate rec_def lp:{{
-  get_rec {{ rec }}.
-  get_def {{ def }}.
-}}.
-
-(* Definition msg_pubkey_right (rec: Type) (def: XDefault rec) := msg_pubkey.
-
-Check  msg_sender.
-
-Definition msg_sender_right (rec: Type) (def: XDefault rec) := msg_sender.
-Check  msg_sender_right.
-
-
-Definition msg_value_right (rec: Type) (def: XDefault rec) := msg_value.
-Definition tvm_pubkey_right (rec: Type) (def: XDefault rec) := tvm_pubkey.
-Definition _now_right (rec: Type) (def: XDefault rec) := \\ now \\.
- *)
 
 Opaque Common.hmapFindWithDefault
-           CommonInstances.addAdjustListPair.
+        CommonInstances.addAdjustListPair
+        N.add N.sub N.leb N.ltb N.eqb Z.eqb.
+
+Definition constructor_exec_computed: forall
+                             (_initialAmount :  uint256) 
+                            (_tokenName :  string) 
+                            (_decimalUnits :  uint8) 
+                            (_tokenSymbol :  string)
+                            (l: LedgerLRecord rec), {t: LedgerLRecord rec | t = constructor_exec _initialAmount _tokenName _decimalUnits _tokenSymbol {$$ l with Ledger_LocalState := default $$}}.
+Proof.        
+    intros. 
+    remember (constructor_exec _initialAmount _tokenName _decimalUnits _tokenSymbol {$$ l with Ledger_LocalState := default $$}).
+
+    destruct l. repeat destruct p.   
+    destruct v. repeat destruct p.
+    destruct c. repeat destruct p.  
+
+    unfold constructor_exec in Heql0.
+    lift_all in Heql0.    
+    compute in Heql0.
+    buint_all in Heql0.
+    symmetry in Heql0.
+    
+    match goal with
+    | Heql0: ?l = l0 |- _ => exact (@exist _ _ l Heql0)
+    end.
+Defined.
+
+Definition constructor_computed_prf  (_initialAmount :  uint256) 
+                            (_tokenName :  string) 
+                            (_decimalUnits :  uint8) 
+                            (_tokenSymbol :  string) (l : LedgerLRecord rec) :
+  proj1_sig (constructor_exec_computed _initialAmount _tokenName _decimalUnits _tokenSymbol l) = 
+  exec_state (Uinterpreter (@constructor rec def _ _ _ _initialAmount _tokenName _decimalUnits _tokenSymbol)) 
+  {$$ l with Ledger_LocalState := default $$}.
+Proof. 
+  rewrite <- constructor_prf.
+  destruct ((constructor_exec_computed _initialAmount _tokenName _decimalUnits _tokenSymbol l)).
+  auto.
+Defined.
+
+
 
 Lemma constructor_set__initialAmount: forall (_initialAmount :  uint256) 
                             (_tokenName :  string) 
                             (_decimalUnits :  uint8) 
                             (_tokenSymbol :  string)
-                            (vmstate: VMStateLRecord), 
-    let l0 := {$$ default with Ledger_VMState := vmstate $$} in
-    let l' := exec_state (Uinterpreter (@constructor rec def _ _ _ _initialAmount _tokenName _decimalUnits _tokenSymbol)) l0 in
+                            (l: LedgerLRecord rec),
+                           (*  (vmstate: VMStateLRecord),  *)
+    let l0 := {$$ l with Ledger_LocalState := default $$} in
+    let l' := exec_state (Uinterpreter (@constructor rec def _ _ _ _initialAmount _tokenName _decimalUnits _tokenSymbol)) l0 in                               
     _totalSupply (l'.(Ledger_MainState)) = _initialAmount.
 Proof.
-    intros. subst l'.
-    rewrite <- constructor_prf.
+    intros. subst l'. subst l0.
+    rewrite <- constructor_computed_prf.
+    
+    destruct l. repeat destruct p.   
+    destruct v. repeat destruct p.
+    destruct c. repeat destruct p.  
+
+    unfold constructor_exec_computed.
+    simpl proj1_sig.
+    unfold LedgerLGetField.
+    unfold ContractLGetField.
+    simpl fold_apply.
+    unfold ClassGeneratorsCommon.CountableMoreAll_obligation_3.
+    unfold LedgerFields_rect.
+    unfold ContractFields_rect.
     auto.
 Qed.
 
@@ -71,13 +87,26 @@ Lemma constructor_set__tokenName: forall (_initialAmount :  uint256)
                             (_tokenName :  string) 
                             (_decimalUnits :  uint8) 
                             (_tokenSymbol :  string)
-                            (vmstate: VMStateLRecord), 
-    let l0 := {$$ default with Ledger_VMState := vmstate $$} in                            
+                            (l: LedgerLRecord rec),
+    let l0 := {$$ l with Ledger_LocalState := default $$} in
     let l' := exec_state (Uinterpreter (@constructor rec def _ _ _ _initialAmount _tokenName _decimalUnits _tokenSymbol)) l0 in
     _name (l'.(Ledger_MainState)) = _tokenName.
 Proof.
-    intros. subst l'.
-    rewrite <- constructor_prf.
+    intros. subst l'. subst l0.
+    rewrite <- constructor_computed_prf.
+    
+    destruct l. repeat destruct p.   
+    destruct v. repeat destruct p.
+    destruct c. repeat destruct p.  
+
+    unfold constructor_exec_computed.
+    simpl proj1_sig.
+    unfold LedgerLGetField.
+    unfold ContractLGetField.
+    simpl fold_apply.
+    unfold ClassGeneratorsCommon.CountableMoreAll_obligation_3.
+    unfold LedgerFields_rect.
+    unfold ContractFields_rect.
     auto.
 Qed.
 
@@ -85,13 +114,26 @@ Lemma constructor_set__decimalUnits: forall (_initialAmount :  uint256)
                             (_tokenName :  string) 
                             (_decimalUnits :  uint8) 
                             (_tokenSymbol :  string)
-                            (vmstate: VMStateLRecord), 
-    let l0 := {$$ default with Ledger_VMState := vmstate $$} in                                
+                            (l: LedgerLRecord rec),
+    let l0 := {$$ l with Ledger_LocalState := default $$} in
     let l' := exec_state (Uinterpreter (@constructor rec def _ _ _ _initialAmount _tokenName _decimalUnits _tokenSymbol)) l0 in
     _decimals (l'.(Ledger_MainState)) = _decimalUnits.
 Proof.
-    intros. subst l'.
-    rewrite <- constructor_prf.
+    intros. subst l'. subst l0.
+    rewrite <- constructor_computed_prf.
+    
+    destruct l. repeat destruct p.   
+    destruct v. repeat destruct p.
+    destruct c. repeat destruct p.  
+
+    unfold constructor_exec_computed.
+    simpl proj1_sig.
+    unfold LedgerLGetField.
+    unfold ContractLGetField.
+    simpl fold_apply.
+    unfold ClassGeneratorsCommon.CountableMoreAll_obligation_3.
+    unfold LedgerFields_rect.
+    unfold ContractFields_rect.
     auto.
 Qed.
 
@@ -99,13 +141,26 @@ Lemma constructor_set__tokenSymbol: forall (_initialAmount :  uint256)
                             (_tokenName :  string) 
                             (_decimalUnits :  uint8) 
                             (_tokenSymbol :  string)
-                            (vmstate: VMStateLRecord), 
-    let l0 := {$$ default with Ledger_VMState := vmstate $$} in 
+                            (l: LedgerLRecord rec),
+    let l0 := {$$ l with Ledger_LocalState := default $$} in
     let l' := exec_state (Uinterpreter (@constructor rec def _ _ _ _initialAmount _tokenName _decimalUnits _tokenSymbol)) l0 in
     _symbol (l'.(Ledger_MainState)) = _tokenSymbol.
 Proof.
-    intros. subst l'.
-    rewrite <- constructor_prf.
+    intros. subst l'. subst l0.
+    rewrite <- constructor_computed_prf.
+    
+    destruct l. repeat destruct p.   
+    destruct v. repeat destruct p.
+    destruct c. repeat destruct p.  
+
+    unfold constructor_exec_computed.
+    simpl proj1_sig.
+    unfold LedgerLGetField.
+    unfold ContractLGetField.
+    simpl fold_apply.
+    unfold ClassGeneratorsCommon.CountableMoreAll_obligation_3.
+    unfold LedgerFields_rect.
+    unfold ContractFields_rect.
     auto.
 Qed.
 
@@ -114,21 +169,27 @@ Lemma constructor_set_sender_balance: forall (_initialAmount :  uint256)
                             (_tokenName :  string) 
                             (_decimalUnits :  uint8) 
                             (_tokenSymbol :  string)
-                            (l: LedgerLRecord rec),
-                            (* (vmstate: VMStateLRecord),  *)
+                            (l: LedgerLRecord rec),                            
     let l0 := {$$ l with Ledger_LocalState := default $$} in
     let l' := exec_state (Uinterpreter (@constructor rec def _ _ _ _initialAmount _tokenName _decimalUnits _tokenSymbol)) l0 in
     let msg_sender := VMState_ι_msg_sender (l.(Ledger_VMState)) in
     (_balances (l'.(Ledger_MainState))) [msg_sender] = _initialAmount.
 Proof.
-    intros. subst l'.
-    rewrite <- constructor_prf.
-
-    destruct l. repeat destruct p.
+    intros. subst l'. subst l0.
+    rewrite <- constructor_computed_prf.
+    
+    destruct l. repeat destruct p.   
     destruct v. repeat destruct p.
-    destruct c. repeat destruct p. 
+    destruct c. repeat destruct p.  
 
-    compute.
+    unfold constructor_exec_computed.
+    simpl proj1_sig.
+    unfold LedgerLGetField.
+    unfold ContractLGetField.
+    simpl fold_apply.
+    unfold ClassGeneratorsCommon.CountableMoreAll_obligation_3.
+    unfold LedgerFields_rect.
+    unfold ContractFields_rect.
 
     rewrite lookup_some_find with (v:=_initialAmount).
     reflexivity.
