src/Proofs/Transfer.v
@@ -15,6 +15,40 @@ Opaque Common.hmapFindWithDefault
         CommonInstances.addAdjustListPair
         N.add N.sub N.leb N.ltb N.eqb Z.eqb.
 
+Definition transfer_exec_computed: forall
+                            (_to :  address)
+                            (_value : uint256)
+                            (l: LedgerLRecord rec), {t: LedgerLRecord rec | t = transfer_exec _to _value {$$ l with Ledger_LocalState := default $$}}.
+Proof.        
+    intros. 
+    remember (transfer_exec _to _value {$$ l with Ledger_LocalState := default $$}).
+
+    destruct l. repeat destruct p.   
+    destruct v. repeat destruct p.
+    destruct c. repeat destruct p.  
+
+    unfold transfer_exec in Heql0.
+    lift_all in Heql0.    
+    compute in Heql0.
+    buint_all in Heql0.
+    symmetry in Heql0.
+    
+    match goal with
+    | Heql0: ?l = l0 |- _ => exact (@exist _ _ l Heql0)
+    end.
+Defined.
+
+Definition transfer_computed_prf  (_to :  address) 
+                         (_value :  uint256) (l : LedgerLRecord rec) :
+  proj1_sig (transfer_exec_computed _to _value l) = 
+  exec_state (Uinterpreter (@transfer rec def _ _ _ _ _to _value)) {$$ l with Ledger_LocalState := default $$}.
+Proof. 
+  rewrite <- transfer_exec_prf.
+  destruct ((transfer_exec_computed _to _value l)).
+  auto.
+Defined.
+
+
 Lemma transfer_set_recepient_balance0: forall (_to :  address) 
                             (_value : uint256)
                             (l: LedgerLRecord rec), 
@@ -25,17 +59,34 @@ Lemma transfer_set_recepient_balance0: forall (_to :  address)
     _to = msg_sender -> 
     (_balances (l'.(Ledger_MainState))) [_to] = recepient_balance0.        
 Proof.        
-    intros. subst l'.
-    rewrite <- transfer_exec_prf.
+    intros. subst l'. subst l0.   
+
+    rewrite <- transfer_computed_prf.
+
     destruct l. repeat destruct p.   
     destruct v. repeat destruct p.
-    destruct c. repeat destruct p.
+    destruct c. repeat destruct p.  
 
-    compute.
+    unfold transfer_exec_computed.
+    simpl proj1_sig.
+    unfold LedgerLGetField.
+    unfold ContractLGetField.
+    simpl fold_apply.
+    unfold ClassGeneratorsCommon.CountableMoreAll_obligation_3.
+    unfold LedgerFields_rect.
+    unfold ContractFields_rect.
+
+    match goal with 
+    | |- _ = ?rhs => let RHS := fresh "rhs" in
+                       let H := fresh "Heqrhs" in   
+                       remember rhs as RHS eqn: H;
+                       compute in H;
+                       buint_all in H;
+                       subst RHS
+    end.
+    
     compute in msg_sender, recepient_balance0.
 
-
-    buint_all.
     match goal with
     | |- context [if ?b then false else true] => remember b
     end.    
@@ -74,38 +125,6 @@ Proof.
 Qed.    
 
 
-Lemma transfer_success: forall (_to :  address) 
-                            (_value : uint256)
-                            (l: LedgerLRecord rec), 
-    let l0 := {$$ l with Ledger_LocalState := default $$} in
-    let r := eval_state (Uinterpreter (@transfer rec def _ _ _ _ _to _value)) l0 in
-    let msg_sender := VMState_ι_msg_sender (l.(Ledger_VMState)) in
-    let msg_sender_balance0 := (_balances (l.(Ledger_MainState))) [msg_sender] in
-    r = if (xIntGeb msg_sender_balance0  _value : bool) then 
-        ControlValue true true
-        else ControlError ERROR_DEFAULT. 
-Proof.
-
-    intros. subst r.
-    rewrite <- transfer_eval_prf.
-    destruct l. repeat destruct p.   
-    destruct v. repeat destruct p.
-    destruct c. repeat destruct p.
-    unfold transfer_eval.    
- 
-    lift_all.
-    compute. 
-    compute in msg_sender, msg_sender_balance0.
-
-    buint_all.
-    match goal with
-    | |- context [if ?b then _ else _] => remember b
-    end.  
-
-    case_eq b; intros; auto.
-Qed.
-
-
 Lemma transfer_set_sender_balance: forall (_to :  address) 
                             (_value : uint256)
                             (l: LedgerLRecord rec), 
@@ -119,16 +138,35 @@ Lemma transfer_set_sender_balance: forall (_to :  address)
         xIntMinus msg_sender_balance0 _value
         else msg_sender_balance0.
 Proof.        
-    intros. subst l'.
-    rewrite <- transfer_exec_prf.
+    intros. subst l'. subst l0.   
+
+    rewrite <- transfer_computed_prf.
+
     destruct l. repeat destruct p.   
     destruct v. repeat destruct p.
-    destruct c. repeat destruct p. 
-    
+    destruct c. repeat destruct p.  
+
+    unfold transfer_exec_computed.
+    simpl proj1_sig.
+    unfold LedgerLGetField.
+    unfold ContractLGetField.
+    simpl fold_apply.
+    unfold ClassGeneratorsCommon.CountableMoreAll_obligation_3.
+    unfold LedgerFields_rect.
+    unfold ContractFields_rect.
+
+    match goal with 
+    | |- _ = ?rhs => let RHS := fresh "rhs" in
+                       let H := fresh "Heqrhs" in   
+                       remember rhs as RHS eqn: H;
+                       compute in H;
+                       buint_all in H;
+                       subst RHS
+    end.
+
+
     compute in msg_sender_balance0, msg_sender.
-    compute. 
- 
-    lift_all.
+    
     match goal with
     | |- context [@addAdjustListPair _ _ _ a ?v _] => remember v
     end.
@@ -165,13 +203,33 @@ Lemma transfer_set_recepient_balance: forall (_to :  address)
         xIntPlus recepient_balance0 _value
         else recepient_balance0.
 Proof.        
-    intros. subst l'.
-    rewrite <- transfer_exec_prf.
+    intros. subst l'. subst l0.   
+
+    rewrite <- transfer_computed_prf.
+
     destruct l. repeat destruct p.   
     destruct v. repeat destruct p.
-    destruct c. repeat destruct p.
+    destruct c. repeat destruct p.  
 
-    compute.
+    unfold transfer_exec_computed.
+    simpl proj1_sig.
+    unfold LedgerLGetField.
+    unfold ContractLGetField.
+    simpl fold_apply.
+    unfold ClassGeneratorsCommon.CountableMoreAll_obligation_3.
+    unfold LedgerFields_rect.
+    unfold ContractFields_rect.
+
+    match goal with 
+    | |- _ = ?rhs => let RHS := fresh "rhs" in
+                       let H := fresh "Heqrhs" in   
+                       remember rhs as RHS eqn: H;
+                       compute in H;
+                       buint_all in H;
+                       subst RHS
+    end.
+    
+    compute in msg_sender_balance0, msg_sender, recepient_balance0.
 
     match goal with
     | |- context [@addAdjustListPair ?K ?V ?H a ?v ?m] => remember (@addAdjustListPair K V H a v m)
@@ -189,7 +247,7 @@ Proof.
     unshelve erewrite lookup_addAdjust.
     refine (BoolEq.pair_eqb_spec (X:=Z) (Y:=XUBInteger 256)).
 
-    subst l3.
+    subst l2.
 
     remember (x10 [_to] ?).
     destruct y.
@@ -216,4 +274,37 @@ Proof.
     refine (BoolEq.pair_eqb_spec (X:=Z) (Y:=XUBInteger 256)).
     setoid_rewrite <- Heqy. reflexivity. 
     assumption.
+Qed.
+
+(* ********************************************************************************************* *)
+
+Lemma transfer_success: forall (_to :  address) 
+                            (_value : uint256)
+                            (l: LedgerLRecord rec), 
+    let l0 := {$$ l with Ledger_LocalState := default $$} in
+    let r := eval_state (Uinterpreter (@transfer rec def _ _ _ _ _to _value)) l0 in
+    let msg_sender := VMState_ι_msg_sender (l.(Ledger_VMState)) in
+    let msg_sender_balance0 := (_balances (l.(Ledger_MainState))) [msg_sender] in
+    r = if (xIntGeb msg_sender_balance0  _value : bool) then 
+        ControlValue true true
+        else ControlError ERROR_DEFAULT. 
+Proof.
+
+    intros. subst r.
+    rewrite <- transfer_eval_prf.
+    destruct l. repeat destruct p.   
+    destruct v. repeat destruct p.
+    destruct c. repeat destruct p.
+    unfold transfer_eval.    
+ 
+    lift_all.
+    compute. 
+    compute in msg_sender, msg_sender_balance0.
+
+    buint_all.
+    match goal with
+    | |- context [if ?b then _ else _] => remember b
+    end.  
+
+    case_eq b; intros; auto.
 Qed.
