src/Proofs/TransferFrom.v
@@ -10,11 +10,44 @@ Import EIP20.
 Require Import Common.
 Require Import EvalExecs.TransferFrom.
 
-
 Opaque Common.hmapFindWithDefault
-        CommonInstances.addAdjustListPair
-        N.add N.sub N.leb N.ltb N.eqb Z.eqb N.pow.
+       CommonInstances.addAdjustListPair
+       N.add N.sub N.leb N.ltb N.eqb Z.eqb N.pow.
 
+Definition transferFrom_exec_computed: forall
+                            (_from :  address)
+                            (_to :  address)
+                            (_value : uint256)
+                            (l: LedgerLRecord rec), {t: LedgerLRecord rec | t = transferFrom_exec _from _to _value {$$ l with Ledger_LocalState := default $$}}.
+Proof.        
+    intros. 
+    remember (transferFrom_exec _from _to _value {$$ l with Ledger_LocalState := default $$}).
+
+    destruct l. repeat destruct p.   
+    destruct v. repeat destruct p.
+    destruct c. repeat destruct p.  
+
+    unfold transferFrom_exec in Heql0.
+    lift_all in Heql0.    
+    compute in Heql0.
+    buint_all in Heql0.
+    symmetry in Heql0.
+    
+    match goal with
+    | Heql0: ?l = l0 |- _ => exact (@exist _ _ l Heql0)
+    end.
+Defined.
+
+Definition transferFrom_computed_prf (_from :  address)
+                         (_to :  address) 
+                         (_value :  uint256) (l : LedgerLRecord rec) :
+  proj1_sig (transferFrom_exec_computed _from _to _value l) = 
+  exec_state (Uinterpreter (@transferFrom rec def _ _ _ _ _from _to _value)) {$$ l with Ledger_LocalState := default $$}.
+Proof. 
+  rewrite <- transferFrom_prf.
+  destruct ((transferFrom_exec_computed _from _to _value l)).
+  auto.
+Defined.
 
 Lemma transferFrom_set_from_balance: forall
                             (_from :  address)
@@ -25,35 +58,46 @@ Lemma transferFrom_set_from_balance: forall
     let l' := exec_state (Uinterpreter (@transferFrom rec def _ _ _ _ _from _to _value)) l0 in
     let msg_sender := VMState_ι_msg_sender (l.(Ledger_VMState)) in
     let _from_balance0 := (_balances (l.(Ledger_MainState))) [_from] in
-     let allowance := (_allowed(l.(Ledger_MainState)))[_from][msg_sender] in
+    let allowance := (_allowed(l.(Ledger_MainState)))[_from][msg_sender] in
     _from <> _to -> 
-(*     (xIntGeb allowance  _value : bool) = true ->
- *)    (_balances (l'.(Ledger_MainState))) [_from] = 
+    (_balances (l'.(Ledger_MainState))) [_from] = 
         if ((xIntGeb _from_balance0  _value : bool)  && (xIntGeb allowance  _value : bool) ) then 
                 xIntMinus _from_balance0 _value
         else _from_balance0.
 Proof.        
-    intros. subst l'.
-    rewrite <- transferFrom_prf.
+    intros. subst l'. subst l0.   
+
+    rewrite <- transferFrom_computed_prf.
 
     destruct l. repeat destruct p.   
     destruct v. repeat destruct p.
     destruct c. repeat destruct p.  
 
-    unfold transferFrom_exec.    
-    lift_all.
+    unfold transferFrom_exec_computed.
+    simpl proj1_sig.
+    unfold LedgerLGetField.
+    unfold ContractLGetField.
+    simpl fold_apply.
+    unfold ClassGeneratorsCommon.CountableMoreAll_obligation_3.
+    unfold LedgerFields_rect.
+    unfold ContractFields_rect.
 
-    compute.
-    compute in _from_balance0, allowance0, msg_sender.  
+    match goal with 
+    | |- _ = ?rhs => let RHS := fresh "rhs" in
+                       let H := fresh "Heqrhs" in   
+                       remember rhs as RHS eqn: H;
+                       compute in H;
+                       buint_all in H;
+                       subst RHS
+    end.
 
-  buint_all.
+    compute in _from_balance0, msg_sender.  
 
     match goal with
     | |- context [if ?b then false else true] => remember b
     end.    
 
     case_eq b; intros; auto.
-
 
     match goal with
     | |- context [if ?b then _ else _] => remember b
@@ -139,20 +183,34 @@ Lemma transferFrom_set_to_balance: forall
                 xIntPlus _to_balance0 _value
         else _to_balance0.
 Proof.        
-    intros. subst l'.
-    rewrite <- transferFrom_prf.
+    intros. subst l'. subst l0.
+
+    rewrite <- transferFrom_computed_prf.
 
     destruct l. repeat destruct p.   
     destruct v. repeat destruct p.
     destruct c. repeat destruct p.  
 
-    unfold transferFrom_exec.    
+    unfold transferFrom_exec_computed.
+    simpl proj1_sig.
+    unfold LedgerLGetField.
+    unfold ContractLGetField.
+    simpl fold_apply.
+    unfold ClassGeneratorsCommon.CountableMoreAll_obligation_3.
+    unfold LedgerFields_rect.
+    unfold ContractFields_rect.
 
-    lift_all.
-    compute.
+    match goal with 
+    | |- _ = ?rhs => let RHS := fresh "rhs" in
+                       let H := fresh "Heqrhs" in   
+                       remember rhs as RHS eqn: H;
+                       compute in H;
+                       buint_all in H;
+                       subst RHS
+    end.
+
     compute in _from_balance0, _to_balance0, allowance0, msg_sender.  
 
-    buint_all.
     match goal with
     | |- context [if ?b then false else true] => remember b
     end.    
@@ -207,22 +265,33 @@ Lemma transferFrom_set_allowed: forall
                 if (xIntGtb MAX_UINT256 allowed0: bool) then xIntMinus allowed0 _value else allowed0
         else allowed0.
 Proof.        
-    intros. subst l'.
-    rewrite <- transferFrom_prf.
+    intros. subst l'. subst l0.
+
+    rewrite <- transferFrom_computed_prf.
 
     destruct l. repeat destruct p.   
     destruct v. repeat destruct p.
     destruct c. repeat destruct p.  
 
-    unfold transferFrom_exec.    
-(*     repeat rewrite exec_if_transit, exec_if_transit2.
- *)
-    lift_all.
-    compute.
+    unfold transferFrom_exec_computed.
+    simpl proj1_sig.
+    unfold LedgerLGetField.
+    unfold ContractLGetField.
+    simpl fold_apply.
+    unfold ClassGeneratorsCommon.CountableMoreAll_obligation_3.
+    unfold LedgerFields_rect.
+    unfold ContractFields_rect.
+
+    match goal with 
+    | |- _ = ?rhs => let RHS := fresh "rhs" in
+                       let H := fresh "Heqrhs" in   
+                       remember rhs as RHS eqn: H;
+                       compute in H;
+                       buint_all in H;
+                       subst RHS
+    end.
+   
     compute in _from_balance0, allowed0, msg_sender.  
-
-
-  buint_all.
 
     match goal with
     | |- context [if ?b then false else true] => remember b
